src/tls/Mem.fst
@@ -1,7 +1,7 @@
-module Mem 
+module Mem
 
 /// Setting a uniform HyperStack-based memory model, and gathering
-/// abbreviations and top-level regions. 
+/// abbreviations and top-level regions.
 
 open FStar.HyperStack.All
 
@@ -10,8 +10,8 @@ open Platform.Bytes
 open Platform.Error
 open TLSError
 
-include FStar.HyperStack 
-include FStar.HyperStack.ST 
+include FStar.HyperStack
+include FStar.HyperStack.ST
 
 module HH = FStar.HyperHeap // avoid if we can
 module HS = FStar.HyperStack
@@ -34,27 +34,35 @@ let is_hs_rgn r    = HH.color r = hs_color
  * Strengthening the predicate because at some places, the code uses HH.parent.
  *)
 let rgn = r:HH.rid{
-  r<>HH.root /\ 
+  r<>HH.root /\
   (forall (s:HH.rid).{:pattern HS.is_eternal_region s} HS.is_above s r ==> HS.is_eternal_region s)}
 
 let tls_rgn   = r:rgn {is_tls_rgn r}
 let epoch_rgn = r:rgn {is_epoch_rgn r}
 let hs_rgn    = r:rgn {is_hs_rgn r}
 
-type fresh_subregion child parent h0 h1 = 
-  stronger_fresh_region child h0 h1 /\ 
+type fresh_subregion child parent h0 h1 =
+  stronger_fresh_region child h0 h1 /\
   HH.extends child parent
 
-type subrgn parent = r:rgn{HH.parent r = parent}  
+type subrgn parent = r:rgn{HH.parent r = parent}
 
 /// Global top-level region for TLS ideal state.
 /// (why do we need a subregion for tables?)
-/// 
+///
 let tls_region: tls_rgn = new_colored_region HH.root tls_color
 
-let tls_tables_region: subrgn tls_region =
-  new_region tls_region
+private let p : r:subrgn tls_region{is_tls_rgn r}
+              & r':subrgn tls_region{is_tls_rgn r' /\ r' `HH.disjoint` r}
+             & r'':subrgn tls_region{is_tls_rgn r'' /\ r'' `HH.disjoint` r' /\ r'' `HH.disjoint` r} =
+  let r = new_colored_region tls_region tls_color in
+  let r' = new_colored_region tls_region tls_color in
+  let r'' = new_colored_region tls_region tls_color in
+  (| r, r', r'' |)
 
-// to be reviewed
-let honest_region: subrgn tls_region = 
-  new_region tls_region
+let tls_tables_region: r:tls_rgn =
+  match p with | (| r, _, _ |) -> r
+let tls_define_region: r:tls_rgn{r `HH.disjoint` tls_tables_region} =
+  match p with | (| _, r, _ |) -> r
+let tls_honest_region: r:tls_rgn{r `HH.disjoint` tls_tables_region /\ r `HH.disjoint` tls_define_region} =
+  match p with | (| _, _, r |) -> r
